Authenticated send and receive function; first draft of events that can be extended by a higher layer

src/lib/communication/DY.Lib.Communication.API.Predicates.fst
@@ -3,26 +3,28 @@ module DY.Lib.Communication.API.Predicates
 open Comparse
 open DY.Core
 open DY.Lib.Crypto.PkEncryption.Split
+open DY.Lib.Crypto.Signature.Split
 open DY.Lib.Event.Typed
 
 open DY.Lib.Communication.API
 
 #set-options "--fuel 0 --ifuel 0 --z3cliopt 'smt.qi.eager_threshold=100'"
 
-(*** Cryptographic Predicates ***)
+(*** PkEnc Predicates ***)
 
 // TODO add higher layer preds as a parameter
-#push-options "--ifuel 2 --fuel 0"
+#push-options "--ifuel 3 --fuel 0"
 val pkenc_crypto_predicates_communication_layer: cusages:crypto_usages -> pkenc_crypto_predicate cusages
 let pkenc_crypto_predicates_communication_layer cusages = {
   pred = (fun tr pk msg ->
-    get_sk_usage pk == PkKey comm_layer_tag empty /\
+    get_sk_usage pk == PkKey comm_layer_pkenc_tag empty /\
       (match parse communication_message msg with
-      | Some {sender; receiver; payload} -> (
+      | Some (CM {sender; receiver; payload}) -> (
         get_sk_label pk == principal_label receiver /\
-        (get_label payload) `can_flow tr` (join (principal_label sender) (principal_label receiver))
+        (get_label payload) `can_flow tr` (join (principal_label sender) (principal_label receiver)) /\
+        event_triggered tr sender (CommConfSendMsg sender receiver payload)
       )
-      | None -> False)
+      | _ -> False)
     );
   pred_later = (fun tr1 tr2 pk msg -> ());
 }
@@ -32,20 +34,77 @@ val pkenc_crypto_predicates_communication_layer_and_tag:
   {|cusages:crypto_usages|} ->
   (string & pkenc_crypto_predicate cusages)
 let pkenc_crypto_predicates_communication_layer_and_tag #cusages = 
-  (comm_layer_tag, pkenc_crypto_predicates_communication_layer cusages)
+  (comm_layer_pkenc_tag, pkenc_crypto_predicates_communication_layer cusages)
+
+(*** Sign Predicates ***)
+
+#push-options "--ifuel 3 --fuel 0"
+val sign_crypto_predicates_communication_layer: cusages:crypto_usages -> sign_crypto_predicate cusages
+let sign_crypto_predicates_communication_layer cusages = {
+  pred = (fun tr vk sig_msg ->
+    get_signkey_usage vk == SigKey comm_layer_sign_tag empty /\
+    (match parse communication_message sig_msg with
+    | Some (CM {sender; receiver; payload}) -> (
+      get_signkey_label vk == principal_label sender /\
+      get_label payload `can_flow tr` public /\
+      event_triggered tr sender (CommAuthSendMsg sender payload)
+    )
+    | _ -> False)
+  );
+  pred_later = (fun tr1 tr2 vk msg -> ());
+}
+#pop-options
+
+val sign_crypto_predicates_communication_layer_and_tag: 
+  {|cusages:crypto_usages|} ->
+  (string & sign_crypto_predicate cusages)
+let sign_crypto_predicates_communication_layer_and_tag #cusages =
+  (comm_layer_sign_tag, sign_crypto_predicates_communication_layer cusages)
 
 val has_communication_layer_invariants:
   crypto_invariants ->
   prop
 let has_communication_layer_invariants cinvs =
-  has_pkenc_predicate cinvs pkenc_crypto_predicates_communication_layer_and_tag
+  has_pkenc_predicate cinvs pkenc_crypto_predicates_communication_layer_and_tag /\
+  has_sign_predicate cinvs sign_crypto_predicates_communication_layer_and_tag
 
 (*** Event Predicates ***)
 
 #push-options "--ifuel 1 --fuel 0"
-let event_predicate_communication_layer {|cinvs:crypto_invariants|} : event_predicate communication_event =
+let event_predicate_communication_layer {|cinvs:crypto_invariants|} (higher_layer_preds:event_predicate communication_event) : event_predicate communication_event =
   fun tr prin e ->
-    match e with
-    | CommunicationLayerSendMsg sender receiver payload -> True
-    | CommunicationLayerReceiveMsg sender receiver payload -> True
+    (
+      match e with
+      | CommConfSendMsg sender receiver payload -> (
+        is_knowable_by (join (principal_label sender) (principal_label receiver)) tr payload
+      )
+      | CommConfReceiveMsg sender receiver payload -> (
+        (
+          event_triggered tr sender (CommConfSendMsg sender receiver payload) /\
+          is_knowable_by (join (principal_label sender) (principal_label receiver)) tr payload
+        ) \/ (
+          is_publishable tr payload
+        )
+      )
+      | CommAuthSendMsg sender payload -> True
+      | CommAuthReceiveMsg sender receiver vk_sender payload -> (
+        event_triggered tr sender (CommAuthSendMsg sender payload) \/
+        is_corrupt tr (get_signkey_label vk_sender)
+      )
+    ) /\
+    higher_layer_preds tr prin e
 #pop-options
+
+val event_predicate_communication_layer_and_tag: 
+  {|cinvs:crypto_invariants|} ->
+  event_predicate communication_event ->
+  (string & compiled_event_predicate)
+let event_predicate_communication_layer_and_tag #cinvs higher_layer_preds =
+  ("DY.Lib.Communication.Event", compile_event_pred #communication_event (event_predicate_communication_layer #cinvs higher_layer_preds))
+
+val has_communication_layer_event_predicates:
+  protocol_invariants ->
+  event_predicate communication_event ->
+  prop
+let has_communication_layer_event_predicates invs higher_layer_preds =
+  has_event_pred invs (event_predicate_communication_layer higher_layer_preds)
